Execution_resources/for_all_correctness.v
@@ -7,44 +7,6 @@ From Views.Execution_resources Require Import sets_of_threads.
 From Views.Execution_resources Require Import collections.
 Require Import PeanoNat.
 
-Proposition induction_step_collection_forall :
-  forall i n v n0 d,
-(forall n' n0, n' < n -> count i (logical_thread_set (v n')) n0 ->
-    count i (logical_thread_set (for_all (v n') d)) n0) ->
-  count i (zip (buildList n (fun i : nat => logical_thread_set (v i)))) n0
--> count i (zip (buildList n (fun i0 : nat => logical_thread_set (for_all (v i0) d))))
-  n0.
-Proof.
-  induction n.
-  + intros. apply H0.
-  + intros. simpl in *.
-  apply cat_count_rev in H0.
-  destruct H0 as [m [m' [H0 [H1 H2]]]]. subst.
-  apply cat_count.
-  apply H. apply le_n. apply H0.
-  apply IHn. intros. apply le_S in H2. apply H with (n0 := n0) in H2. apply H2. apply H3.
-  apply H1.
-Qed.
-
-Proposition induction_step_collection_forall_physical :
-  forall i n v n0 d f,
-(forall n' n0, n' < n -> count i (physical_thread_set (v n') f) n0 ->
-    count i (physical_thread_set (for_all (v n') d) f) n0) ->
-  count i (zip (buildList n (fun i : nat => physical_thread_set (v i) f))) n0
--> count i (zip (buildList n (fun i0 : nat => physical_thread_set (for_all (v i0) d) f)))
-  n0.
-Proof.
-  induction n.
-  + intros. apply H0.
-  + intros. simpl in *.
-  apply cat_count_rev in H0.
-  destruct H0 as [m [m' [H0 [H1 H2]]]]. subst.
-  apply cat_count.
-  apply H. apply le_n. apply H0.
-  apply IHn. intros. apply le_S in H2. apply H with (n0 := n0) in H2. apply H2. apply H3.
-  apply H1.
-Qed.
-
 Proposition for_all_correct :
   (** If e.forall(d) gives a valid output, then it preserves the number of logical threads *)
   forall i e d m,
